\section*{H4}

\subsection*{a)}

	\subsubsection*{IA}
		FÃ¼r $q \in Q, u = \varepsilon$ gilt $\hat{\delta}(q,uv) =  \hat{\delta}(q,v) = \hat{\delta}(\hat{\delta}(q,u),v)$ 

	\subsubsection*{IV}
	Sei $u \in \Sigma^*$
	
	Und es gilt 	
	$\forall q \in Q:\hat{\delta}(q,uv) =  \hat{\delta}(\hat{\delta}(q,u),v)$ 
	
	\subsubsection*{IS}
	
	Sei $a \in \Sigma$
	dann gilt:
	$\hat{\delta}(q,auv)
	= \hat{\delta}(\delta(q,a),uv)
	= \hat{\delta}(\hat{\delta}(\delta(q,a),u),v)
	= \hat{\delta}(\hat{\delta}(q,au),v)$ 
	  


\subsection*{b)}

\subsection*{c)}

